monadproofs/proofs/execproofs/exec_transaction.v
@@ -1,0 +1,59 @@
+Require Import monad.proofs.misc.
+Require Import monad.proofs.libspecs.
+Require Import monad.proofs.evmopsem.
+Import linearity.
+Require Import bedrock.auto.invariants.
+Require Import bedrock.auto.cpp.proof.
+
+Require Import bedrock.auto.cpp.tactics4.
+Require Import monad.asts.ext.
+Require Import monad.proofs.exec_specs.
+
+Opaque libspecs.optionR.
+
+Section with_Sigma.
+  Context `{Sigma:cpp_logic} {CU: genv}.
+           (*   hh = @has_own_monpred thread_info _Σ fracR (@cinv_inG _Σ (@cpp_has_cinv thread_info _Σ Sigma)) *)
+  Context  {MODd : ext.module ⊧ CU}.
+
+  Set Nested Proofs Allowed.
+  Set Printing Coercions.
+  #[global] Instance learnOpt a b c d e a1 b1 c1 d1 e1: Learnable (@libspecs.optionR _ _ _ _ a b c d e) (@libspecs.optionR _ _ _ _ a1 b1 c1 d1 e1) [a=a1] := ltac:(solve_learnable).
+  
+Lemma prf: denoteModule module
+             ** (opt_reconstr TransactionResult resultT)
+             ** tvector_spec
+             ** reset_promises
+             ** (fork_taskg (Nscoped (Ninst "monad::execute_transactions(const monad::Block&, monad::fiber::PriorityPool&, const monad::Chain&, const monad::BlockHashBuffer&, monad::BlockState &)" [Avalue (Eint 11 "enum evmc_revision")]) (Nanon 0)))
+             ** vector_op_monad
+             ** recover_sender
+             ** wait_for_promise
+             ** set_value
+             ** destrop
+             ** destr_res
+             ** (has_value "evmc::address")
+             ** (value "evmc::address")
+             |-- ext1.
+Proof using MODd.
+  verify_spec'.
+  go; try (ego; fail).
+  cpp.spec (
+          (Ninst
+             (Nscoped (Nglobal (Nid "monad"))
+                (Nfunction function_qualifiers.N (Nf "execute_impl")
+                   [Tref (Tconst (Tnamed (Nscoped (Nglobal (Nid "monad")) (Nid "Chain")))); "unsigned long"%cpp_type;
+                    Tref (Tconst (Tnamed (Nscoped (Nglobal (Nid "monad")) (Nid "Transaction"))));
+                    Tref (Tconst (Tnamed (Nscoped (Nglobal (Nid "evmc")) (Nid "address"))));
+                    Tref (Tconst (Tnamed (Nscoped (Nglobal (Nid "monad")) (Nid "BlockHeader"))));
+                    Tref (Tconst (Tnamed (Nscoped (Nglobal (Nid "monad")) (Nid "BlockHashBuffer"))));
+                    Tref (Tnamed (Nscoped (Nglobal (Nid "monad")) (Nid "BlockState")));
+                    Tref
+                      (Tnamed
+                         (Ninst (Nscoped (Nscoped (Nglobal (Nid "boost")) (Nid "fibers")) (Nid "promise"))
+                            [Atype "void"]))]))
+             [Avalue (Eint 11 (Tenum (Nglobal (Nid "evmc_revision"))))])) as fff inline.
+  slauto.
+
+Abort.
+
+End with_Sigma.
